New proof of is_wp in progress.

wp.v
@@ -1,6 +1,27 @@
 Require Import List.
 Require Import Omega.
 
+Lemma app_last {A}:
+  forall (l1 l2:list A) d,
+  l2 <> nil -> last (l1 ++ l2) d = last l2 d.
+Proof.
+  intros l1 l2 d l2_non_nil; induction l1.
+  + auto.
+  + cut (length (l1 ++ l2) > 0).
+    {
+      rewrite <-app_comm_cons; simpl; destruct (l1 ++ l2).
+      + simpl; intros; omega.
+      + rewrite IHl1; auto.
+    }
+    cut (length l2 > 0).
+    {
+      intros; rewrite app_length; omega.
+    }
+    destruct l2.
+    - exfalso; apply l2_non_nil; auto.
+    - simpl; omega.
+Qed.
+
 Inductive paren :=
   | open
   | close.
@@ -35,4 +56,104 @@ Lemma wp_implies_is_wp: forall l, wp l -> is_wp l = true.
 Proof.
   intros; unfold is_wp; rewrite <-app_nil_r with (l := l).
   rewrite wp_implies_no_change by auto; auto.
+Qed.
+
+Fixpoint rep_open (n:nat) :=
+  match n with
+  | 0 => nil
+  | S k => open :: (rep_open k)
+  end.
+
+Lemma rep_open_split_last:
+  forall n l, rep_open n ++ open :: l = rep_open (S n) ++ l.
+Proof.
+  intros; induction n.
+  + simpl; auto.
+  + simpl rep_open in *; repeat rewrite <-app_comm_cons; rewrite IHn.
+    repeat rewrite <-app_comm_cons; auto.
+Qed.
+
+Lemma wp_non_nil_ends_close:
+  forall l d, wp l -> l <> nil -> last l d = close.
+Proof.
+  intros l d wp_l l_non_nil.
+  induction wp_l.
+  + exfalso; apply l_non_nil; auto.
+  + rewrite app_comm_cons, app_last.
+    - auto.
+    - discriminate.
+  + destruct l1, l2.
+    - simpl in *; exfalso; apply l_non_nil; auto.
+    - rewrite app_nil_l, IHwp_l2; auto.
+    - rewrite app_nil_r, IHwp_l1; auto; discriminate.
+    - rewrite app_last.
+      * rewrite IHwp_l2; auto; discriminate.
+      * discriminate.
+Qed.
+
+Lemma open_close_keeps_wp:
+  forall l n, wp ((rep_open n) ++ l) -> wp ((rep_open (S n)) ++ close :: l).
+Proof.
+  assert (forall (p:paren) l, p :: nil ++ l = p :: l) as cons_eq by auto.
+  assert (wp (open :: close :: nil)) as wp_open_close by
+    (rewrite <-cons_eq; apply wp_p, wp_e).
+  cut (forall m l n,
+       length l <= m ->
+       wp (rep_open n ++ l) ->
+       wp (rep_open (S n) ++ close :: l)).
+  {
+    intros H l n; apply H with (m := length l); omega.
+  }
+  induction m.
+  {
+    destruct l, n; simpl; intros; try omega.
+    + apply wp_open_close.
+    + rewrite app_comm_cons; apply wp_p; rewrite <-app_nil_r; auto.
+  }
+  {
+    destruct l, n; simpl; intros.
+    + apply wp_open_close.
+    + rewrite app_comm_cons; apply wp_p; rewrite <-app_nil_r; auto.
+    + rewrite <-cons_eq with (p := open).
+      rewrite <-cons_eq with (p := close).
+      do 2 rewrite app_comm_cons; rewrite app_assoc, <-app_comm_cons, cons_eq.
+      apply wp_c.
+      - apply wp_open_close.
+      - auto.
+    + admit. (** FIXME **)
+  }
+Qed.
+
+Lemma is_wp_implies_wp_aux:
+  forall l n, is_wp_aux l n = true -> wp ((rep_open n) ++ l).
+Proof.
+  induction l.
+  {
+    simpl; intros; destruct n.
+    + simpl; apply wp_e.
+    + discriminate.
+  }
+  {
+    intros; destruct a.
+    + rewrite rep_open_split_last; apply IHl; simpl in *; auto.
+    + destruct n.
+      - simpl in *; discriminate.
+      - simpl in *; apply open_close_keeps_wp, IHl; auto.
+  }
+Qed.
+
+Lemma is_wp_implies_wp: forall l, is_wp l = true -> wp l.
+Proof.
+  unfold is_wp; intros.
+  assert (nil = rep_open 0) as rep_open_0_is_nil by auto.
+  rewrite <-app_nil_l, rep_open_0_is_nil.
+  apply is_wp_implies_wp_aux; auto.
+Qed.
+
+Lemma is_wp_works:
+  forall l, is_wp l = true <-> wp l.
+Proof.
+  split.
+  + apply is_wp_implies_wp.
+  + apply wp_implies_is_wp.
 Qed.
